src/tls/TLS.Handshake.fst
@@ -29,6 +29,7 @@ module HSM = HandshakeMessages
 
 module Client = TLS.Handshake.Client
 module Server = TLS.Handshake.Server
+module Receive = TLS.Handshake.Receive 
 module PF = TLS.Handshake.ParseFlights
 
 module LP = LowParse.Low.Base
